Library/General/Order.sw
@@ -105,10 +105,10 @@ proof Isa unstrictify_Obligation_subtype
   apply (simp add: bij_ON_def inj_on_def surj_on_def Ball_def 
                    mem_def Order__strictify_def, safe)
   apply (thin_tac "refl x", simp add: refl_on_def, case_tac "a=b", simp)
-  apply (thin_tac "?P", simp add: expand_set_eq, 
+  apply (thin_tac "?P", simp add:set_eq_iff, 
          drule_tac x=a in spec, drule_tac x=b in  spec, simp)
   apply (thin_tac "refl xa", simp add: refl_on_def, case_tac "a=b", simp)
-  apply (thin_tac "?P", simp add: expand_set_eq, 
+  apply (thin_tac "?P", simp add:set_eq_iff, 
          drule_tac x=a in spec, drule_tac x=b in  spec, simp)
   apply (rule_tac x="x \<union> Id" in bexI, simp_all add: mem_def)
   apply (auto simp add: irrefl_def)
